---
layout: clrs-solution
title:  "Exercise 2.3-3"
---
**Use mathematical induction to show that when *n* is an exact power of 2, the solution of the recurrence**

**T(n) = { 2, if n = 2**

**T(n) = { 2T(n/2) + n, if n = 2<sup>k</sup>, for k > 1**

**is T(n) = *n*lg*n***

In the base case, *k* = 1, and so *n* = 2<sup>1</sup>. *T*(*n*) = *n*lg*n* = 2·lg(2<sup>1</sup>) = 2·1 = 2. 

Next we suppose this holds for any *k* > 1, and will show that it also holds for any *k* + 1:

*T*(*n*/2) + *n* = *n*lg*n*

2[(2<sup>*k* + 1</sup>/2)·lg(2<sup>*k* + 1</sup>/2)] + 2<sup>*k* + 1</sup> = 2<sup>*k* + 1</sup>lg2<sup>*k* + 1</sup>

2{[2<sup>*k* + 1</sup>/2]·[lg(2<sup>*k* + 1</sup>/2) - lg2] + 2<sup>*k* + 1</sup> = 2<sup>*k* + 1</sup>(*k* + 1)

2{[2<sup>*k* + 1</sup>/2]·[*k* + 1 - 1] + 2<sup>*k* + 1</sup> = 2<sup>*k* + 1</sup>(*k* + 1)

2<sup>*k* + 1</sup>·*k* + 2<sup>*k* + 1</sup> = 2<sup>*k* + 1</sup>(*k* + 1)

2<sup>*k* + 1</sup>(*k* + 1) = 2<sup>*k* + 1</sup>(*k* + 1)